Created streamlined inlining theorems using BaseModuleWf.

PPlusProperties.v
@@ -2061,6 +2061,29 @@ Proof.
   eauto using StrongPPlusTraceInclusion_PPlusTraceInclusion, PPlusStrongTraceInclusion_inlining_Rules_r.
 Qed.
 
+
+Lemma WfBaseMod_Rule_inlined m f rn:
+  WfBaseModule m ->
+  In f (getMethods m) ->
+  WfBaseModule (inlineSingle_Rule_BaseModule f rn m).
+Proof.
+  intros.
+  specialize (WfMod_Rule_inlined (m:=m) f rn); intros.
+  assert (WfMod m) as TMP;[constructor; auto|specialize (H1 TMP H0); clear TMP].
+  inversion H1; auto.
+Qed.
+
+Definition inlineSingle_Rule_BaseModuleWf {f} rn {m: BaseModuleWf} (inMeths: In f (getMethods m)):=
+  Build_BaseModuleWf (WfBaseMod_Rule_inlined f rn (wfBaseModule m) inMeths).
+
+Theorem TraceInclusion_inlining_Rules_Wf_r {f} {m : BaseModuleWf} rn
+        (inMeths: In f (getMethods m)):
+  TraceInclusion m (inlineSingle_Rule_BaseModuleWf rn inMeths).
+Proof.
+  simpl; apply TraceInclusion_inlining_Rules_r; eauto.
+  constructor; apply wfBaseModule.
+Qed.
+
 Lemma ProjT1_inline_eq (f g : DefMethT):
   (projT1 (snd g)) = (projT1 (snd (inlineSingle_Meth f g))).
 Proof.
@@ -2820,6 +2843,28 @@ Proof.
   eauto using StrongPPlusTraceInclusion_PPlusTraceInclusion, PPlusStrongTraceInclusion_inlining_Meth_r.
 Qed.
 
+Lemma WfBaseMod_Meth_inlined m f gn :
+  (WfBaseModule m) ->
+  In f (getMethods m) ->
+  (WfBaseModule (inlineSingle_Meth_BaseModule f gn m)).
+Proof.
+  intros.
+  specialize (WfMod_Meth_inlined (m:=m) f gn); intro.
+  assert (WfMod m) as TMP;[constructor; auto|specialize (H1 TMP H0); clear TMP].
+  inv H1; auto.
+Qed.
+
+Definition inlineSingle_Meth_BaseModuleWf {f} {m: BaseModuleWf} gn (inMeths: In f (getMethods m)):=
+  Build_BaseModuleWf (WfBaseMod_Meth_inlined f gn (wfBaseModule m) inMeths).
+
+Theorem TraceInclusion_inlining_Meth_Wf_r {f} {m : BaseModuleWf} rn
+        (inMeths: In f (getMethods m)):
+  TraceInclusion m (inlineSingle_Meth_BaseModuleWf rn inMeths).
+Proof.
+  simpl; apply TraceInclusion_inlining_Meth_r; eauto.
+  constructor; apply wfBaseModule.
+Qed.
+
 Section Rel.
   Variable A B: Type.
   Variable f: B -> A  -> A.
@@ -3071,6 +3116,82 @@ Proof.
     apply TraceInclusion_refl.
 Qed.
 
+Lemma WfBaseMod_inline_nth_Meth m f i:
+  In f (getMethods m) ->
+  (WfBaseModule m) ->
+  (WfBaseModule (BaseMod (getRegisters m) (getRules m) (transform_nth_right (inlineSingle_Meth f) i (getMethods m)))).
+Proof.
+  intros.
+  destruct (lt_dec i (length (getMethods m))).
+  - pose proof H0 as H0'.
+    destruct H0 as [? [? [NoDupMeths [NoDupRegisters NoDupRle]]]].
+    simpl in *.
+    specialize (inlineSingle_Meth_transform_nth f _ NoDupMeths l) as TMP; dest.
+    rewrite H3.
+    assert (In f (transform_nth_right (inlineSingle_Meth f) i (getMethods m)));
+      [apply inline_Meth_not_transformed; auto|].
+    assert (WfMod m) as P1; [constructor; auto|].
+    specialize (WfMod_Meth_inlined _ (fst x) P1 H) as P2.
+    unfold inlineSingle_Meth_BaseModule in P2; simpl in *.
+    inv P2; eauto.
+  - apply Nat.nlt_ge in n.
+    rewrite inlineSingle_transform_gt; auto.
+    assert (WfMod m) as P1;[constructor; auto| apply (WfMod_WfBaseMod_flat P1)].
+Qed.
+
+Definition inline_nth_Meth_BaseModuleWf {f} {m : BaseModuleWf} i
+           (inMeths : In f (getMethods m)):=
+  (Build_BaseModuleWf (WfBaseMod_inline_nth_Meth f i inMeths (wfBaseModule m))).
+
+Theorem inline_meth_transform_Wf {f} {m : BaseModuleWf} i (inMeths : In f (getMethods m)):
+    TraceInclusion m (inline_nth_Meth_BaseModuleWf i inMeths).
+Proof.
+  intros; simpl.
+  specialize (_TraceInclusion_flatten_r m) as P1.
+  specialize (wfMod (flattened_ModWf m)) as P2; simpl in *.
+  unfold flatten, getFlat in *; simpl in *.
+  specialize (inline_meth_transform f P2 inMeths i) as P3.
+  eauto using TraceInclusion_trans.
+Qed.
+
+Lemma WfBaseMod_inline_all_Meth m f xs:
+  In f (getMethods m) ->
+  (WfBaseModule m) ->
+  (WfBaseModule (BaseMod (getRegisters m) (getRules m) (fold_right (transform_nth_right (inlineSingle_Meth f)) (getMethods m) xs))).
+Proof.
+  intros.
+  assert (WfMod (Base m)) as P1;[constructor; auto|].
+  specialize (WfMod_WfBaseMod_flat P1) as P2.
+  unfold getFlat in P2; simpl in *.
+  assert (WfMod (Base (BaseMod (getRegisters m) (getRules m) (getMethods m)))) as P3;
+    [constructor; auto|].
+  specialize (WfMod_inline_all_Meth f xs H P3) as P4.
+  inv P4; auto.
+Qed.
+
+Definition inline_all_Meth_BaseModuleWf {f} {m : BaseModuleWf} xs
+           (inMeths : In f (getMethods m)):=
+  (Build_BaseModuleWf (WfBaseMod_inline_all_Meth f xs inMeths (wfBaseModule m))).
+
+Lemma WfBaseMod_inline_all_Rule m f xs:
+  In f (getMethods m) ->
+  (WfBaseModule m) ->
+  (WfBaseModule (BaseMod (getRegisters m) (fold_right (transform_nth_right (inlineSingle_Rule f)) (getRules m) xs) (getMethods m))).
+Proof.
+  intros.
+  assert (WfMod (Base m)) as P1;[constructor; auto|].
+  specialize (WfMod_WfBaseMod_flat P1) as P2.
+  unfold getFlat in P2; simpl in *.
+  assert (WfMod (Base (BaseMod (getRegisters m) (getRules m) (getMethods m)))) as P3;
+    [constructor; auto|].
+  specialize (WfMod_inline_all_Rule f xs H P3) as P4.
+  inv P4; auto.
+Qed.
+
+Definition inline_all_Rule_BaseModuleWf {f} {m : BaseModuleWf} xs
+           (inMeths : In f (getMethods m)):=
+  (Build_BaseModuleWf (WfBaseMod_inline_all_Rule f xs inMeths (wfBaseModule m))).
+
 Theorem inline_rule_transform f regs rules meths:
   (WfMod (Base (BaseMod regs rules meths))) ->
   In f meths ->
@@ -3090,6 +3211,41 @@ Proof.
   - apply Nat.nlt_ge in n.
     rewrite inlineSingle_transform_gt; auto.
     apply TraceInclusion_refl.
+Qed.
+
+Lemma WfBaseMod_inline_nth_Rule m f i:
+  In f (getMethods m) ->
+  (WfBaseModule m) ->
+  (WfBaseModule (BaseMod (getRegisters m) (transform_nth_right (inlineSingle_Rule f) i (getRules m)) (getMethods m))).
+Proof.
+  intros.
+  destruct (lt_dec i (length (getRules m))).
+  - pose proof H0 as H0'.
+    destruct H0 as [? [? [NoDupMeths [NoDupRegisters NoDupRle]]]].
+    specialize (inlineSingle_Rule_transform_nth f _ NoDupRle l) as TMP; dest.
+    rewrite H3.
+    assert (WfMod m) as P1; [constructor; auto|].
+    specialize (WfMod_Rule_inlined _ (fst x) P1 H) as P2.
+    unfold inlineSingle_Rule_BaseModule in P2; simpl in *.
+    inv P2; eauto.
+  - apply Nat.nlt_ge in n.
+    rewrite inlineSingle_transform_gt; auto.
+    assert (WfMod m) as P1;[constructor; auto| apply (WfMod_WfBaseMod_flat P1)].
+Qed.
+
+Definition inline_nth_Rule_BaseModuleWf {f} {m : BaseModuleWf} i
+           (inMeths : In f (getMethods m)):=
+  (Build_BaseModuleWf (WfBaseMod_inline_nth_Rule f i inMeths (wfBaseModule m))).
+
+Theorem inline_rule_transform_Wf {f} {m : BaseModuleWf} i (inMeths : In f (getMethods m)):
+    TraceInclusion m (inline_nth_Rule_BaseModuleWf i inMeths).
+Proof.
+  intros; simpl.
+  specialize (_TraceInclusion_flatten_r m) as P1.
+  specialize (wfMod (flattened_ModWf m)) as P2; simpl in *.
+  unfold flatten, getFlat in *; simpl in *.
+  specialize (inline_rule_transform f P2 inMeths i) as P3.
+  eauto using TraceInclusion_trans.
 Qed.
 
 Section inlineSingle_nth.
@@ -3125,17 +3281,66 @@ Section inlineSingle_nth.
   Qed.
 End inlineSingle_nth.
 
+Theorem inline_meth_fold_right_Wf {f} {m : BaseModuleWf} xs (inMeth : In f (getMethods m)):
+  TraceInclusion m (inline_all_Meth_BaseModuleWf xs inMeth).
+Proof.
+  specialize (_TraceInclusion_flatten_r m) as P1.
+  simpl in *; unfold flatten, getFlat in P1; simpl in *.
+  assert (WfMod m) as TMP;[constructor; apply wfBaseModule
+                          |specialize (_WfMod_getFlat TMP) as P2; clear TMP].
+  specialize (inline_meth_fold_right f P2 xs inMeth) as P3.
+  eauto using TraceInclusion_trans.
+Qed.
+
+Theorem inline_rule_fold_right_Wf {f} {m : BaseModuleWf} xs (inMeth : In f (getMethods m)):
+  TraceInclusion m (inline_all_Rule_BaseModuleWf xs inMeth).
+Proof.
+  specialize (_TraceInclusion_flatten_r m) as P1.
+  simpl in *; unfold flatten, getFlat in P1; simpl in *.
+  assert (WfMod m) as TMP;[constructor; apply wfBaseModule
+                          |specialize (_WfMod_getFlat TMP) as P2; clear TMP].
+  specialize (inline_rule_fold_right f P2 xs inMeth) as P3.
+  eauto using TraceInclusion_trans.
+Qed.
+
 Theorem TraceInclusion_inline_BaseModule_rules regs rules meths f:
   (WfMod (Base (BaseMod regs rules meths))) ->
   In f meths ->
   TraceInclusion (Base (BaseMod regs rules meths)) (Base (BaseMod regs (map (inlineSingle_Rule f) rules) meths)).
 Proof.
   intros.
-  unfold inlineSingle_BaseModule.
   specialize (inline_rule_fold_right f H (0 upto (length rules)) H0) as P1.
   specialize (WfMod_inline_all_Rule _ (0 upto (length rules)) H0 H) as P2.
   repeat rewrite map_fold_right_eq in *.
   assumption.
+Qed.
+
+Lemma WfBaseMod_inline_BaseModule_Rules m f:
+  In f (getMethods m) ->
+  WfBaseModule m ->
+  WfBaseModule (BaseMod (getRegisters m) (map (inlineSingle_Rule f) (getRules m)) (getMethods m)).
+Proof.
+  intros.
+  assert (WfMod m) as TMP;[constructor; auto|specialize (_WfMod_getFlat TMP) as P1; clear TMP].
+  specialize (WfMod_inline_all_Rule _ (0 upto (length (getRules m))) H P1) as P2.
+  repeat rewrite map_fold_right_eq in *; simpl in *.
+  inv P2; auto.
+Qed.
+
+Definition inline_BaseModule_rules_BaseModuleWf {f} {m : BaseModuleWf}
+           (inMeth : In f (getMethods m)) :=
+  Build_BaseModuleWf (WfBaseMod_inline_BaseModule_Rules _ inMeth (wfBaseModule m)).
+
+Theorem TraceInclusion_inline_BaseModule_rules_Wf {f} {m : BaseModuleWf}
+        (inMeth : In f (getMethods m)):
+  TraceInclusion m (inline_BaseModule_rules_BaseModuleWf inMeth).
+Proof.
+  specialize (_TraceInclusion_flatten_r m) as P1.
+  simpl in *; unfold flatten, getFlat in P1; simpl in *.
+  assert (WfMod m) as TMP;[constructor; apply wfBaseModule
+                          |specialize (_WfMod_getFlat TMP) as P2; clear TMP].
+  specialize (TraceInclusion_inline_BaseModule_rules f P2 inMeth) as P3.
+  eauto using TraceInclusion_trans.
 Qed.
 
 Theorem TraceInclusion_inline_BaseModule_meths regs rules meths f:
@@ -3150,6 +3355,34 @@ Proof.
   assumption.
 Qed.
 
+Lemma WfBaseMod_inline_BaseModule_Meths m f:
+  In f (getMethods m) ->
+  WfBaseModule m ->
+  WfBaseModule (BaseMod (getRegisters m) (getRules m) (map (inlineSingle_Meth f) (getMethods m))).
+Proof.
+  intros.
+  assert (WfMod m) as TMP;[constructor; auto|specialize (_WfMod_getFlat TMP) as P1; clear TMP].
+  specialize (WfMod_inline_all_Meth _ (0 upto (length (getMethods m))) H P1) as P2.
+  repeat rewrite map_fold_right_eq in *; simpl in *.
+  inv P2; auto.
+Qed.
+
+Definition inline_BaseModule_meths_BaseModuleWf {f} {m : BaseModuleWf}
+           (inMeth : In f (getMethods m)) :=
+  Build_BaseModuleWf (WfBaseMod_inline_BaseModule_Meths _ inMeth (wfBaseModule m)).
+
+Theorem TraceInclusion_inline_BaseModule_meths_Wf {f} {m : BaseModuleWf}
+        (inMeth : In f (getMethods m)):
+  TraceInclusion m (inline_BaseModule_meths_BaseModuleWf inMeth).
+Proof.
+  specialize (_TraceInclusion_flatten_r m) as P1.
+  simpl in *; unfold flatten, getFlat in P1; simpl in *.
+  assert (WfMod m) as TMP;[constructor; apply wfBaseModule
+                          |specialize (_WfMod_getFlat TMP) as P2; clear TMP].
+  specialize (TraceInclusion_inline_BaseModule_meths f P2 inMeth) as P3.
+  eauto using TraceInclusion_trans.
+Qed.
+
 Theorem TraceInclusion_inline_BaseModule_all regs rules meths f:
   (WfMod (Base (BaseMod regs rules meths))) ->
   In f meths ->
@@ -3162,6 +3395,32 @@ Proof.
   specialize (TraceInclusion_inline_BaseModule_meths f P2 H0) as P3.
   repeat rewrite map_fold_right_eq in *.
   apply (TraceInclusion_trans P1 P3).
+Qed.
+
+Lemma WfBaseMod_inlineSingle_BaseModule m f:
+  In f (getMethods m) ->
+  WfBaseModule m ->
+  WfBaseModule (inlineSingle_BaseModule f (getRegisters m) (getRules m) (getMethods m)).
+Proof.
+  intros.
+  unfold inlineSingle_BaseModule.
+  specialize (WfBaseMod_inline_BaseModule_Rules f H H0) as P1.
+  assert (In f (getMethods ((BaseMod (getRegisters m) (map (inlineSingle_Rule f) (getRules m)) (getMethods m))))) as P2;[simpl; auto|].
+  apply (WfBaseMod_inline_BaseModule_Meths f P2 P1).
+Qed.
+
+Definition inlineSingle_BaseModuleWf {f} {m : BaseModuleWf} (inMeth : In f (getMethods m)):=
+  Build_BaseModuleWf (WfBaseMod_inlineSingle_BaseModule _ inMeth (wfBaseModule m)).
+
+Theorem TraceInclusion_inline_BaseModule_all_Wf {f} {m : BaseModuleWf}
+        (inMeth : In f (getMethods m)):
+  TraceInclusion m (inlineSingle_BaseModuleWf inMeth).
+Proof.
+  specialize (_TraceInclusion_flatten_r m) as P1.
+  specialize (wfMod (flattened_ModWf m)) as P2.
+  simpl in *; unfold flatten, getFlat in *; simpl in *.
+  specialize (TraceInclusion_inline_BaseModule_all _ P2 inMeth) as P3.
+  eauto using TraceInclusion_trans.
 Qed.
 
 Section inline_all_all.
@@ -3183,6 +3442,30 @@ Section inline_all_all.
       eapply nth_error_In; eauto.
   Qed.
 
+  Lemma WfBaseMod_inlineSingle_Rules_pos m n:
+    WfBaseModule m ->
+    WfBaseModule (BaseMod (getRegisters m) (inlineSingle_Rules_pos (getMethods m) n (getRules m)) (getMethods m)).
+  Proof.
+    intros.
+    assert (WfMod m) as P1;[constructor; auto|apply _WfMod_getFlat in P1].
+    unfold getFlat in P1; simpl in *.
+    specialize (TraceInclusion_inlineSingle_pos_Rules P1 n) as TMP; dest.
+    inversion H0; auto.
+  Qed.
+
+  Definition inlineSingle_Rules_pos_BaseModuleWf (m : BaseModuleWf) n :=
+    Build_BaseModuleWf (WfBaseMod_inlineSingle_Rules_pos n (wfBaseModule m)).
+
+  Theorem TraceInclusion_inlineSingle_pos_Rules_Wf (m : BaseModuleWf) n :
+    TraceInclusion m (inlineSingle_Rules_pos_BaseModuleWf m n).
+  Proof.
+    specialize (_TraceInclusion_flatten_r m) as P1.
+    specialize (wfMod (flattened_ModWf m)) as P2.
+    simpl in *; unfold flatten, getFlat in *; simpl in *.
+    specialize (TraceInclusion_inlineSingle_pos_Rules P2 n) as TMP; dest.
+    eauto using TraceInclusion_trans.
+  Qed.
+  
   Theorem TraceInclusion_inlineAll_pos_Rules regs rules meths:
     (WfMod (Base (BaseMod regs rules meths))) ->
     (WfMod (Base (BaseMod regs (inlineAll_Rules meths rules) meths))) /\
@@ -3197,6 +3480,30 @@ Section inline_all_all.
     destruct n; simpl in *; auto.
     split; auto.
     eapply TraceInclusion_trans; eauto.
+  Qed.
+  
+  Lemma WfBaseMod_inlineAll_Rules m :
+    WfBaseModule m ->
+    WfBaseModule (BaseMod (getRegisters m) (inlineAll_Rules (getMethods m) (getRules m)) (getMethods m)).
+  Proof.
+    intros.
+    assert (WfMod m) as P1;[constructor; auto|apply _WfMod_getFlat in P1].
+    unfold getFlat in P1; simpl in *.
+    specialize (TraceInclusion_inlineAll_pos_Rules P1) as TMP; dest.
+    inversion H0; auto.
+  Qed.
+
+  Definition inlineAll_Rules_BaseModuleWf (m : BaseModuleWf) :=
+    Build_BaseModuleWf (WfBaseMod_inlineAll_Rules (wfBaseModule m)).
+
+  Theorem TraceInclusion_inlineAll_pos_Rules_Wf (m : BaseModuleWf) :
+    TraceInclusion m (inlineAll_Rules_BaseModuleWf m).
+  Proof.
+    specialize (_TraceInclusion_flatten_r m) as P1.
+    specialize (wfMod (flattened_ModWf m)) as P2.
+    simpl in *; unfold flatten, getFlat in *; simpl in *.
+    specialize (TraceInclusion_inlineAll_pos_Rules P2) as TMP; dest.
+    eauto using TraceInclusion_trans.
   Qed.
   
   Theorem TraceInclusion_inlineSingle_pos_Meths regs rules meths:
@@ -3217,6 +3524,30 @@ Section inline_all_all.
       eapply nth_error_In; eauto.
   Qed.
 
+  Lemma WfBaseMod_inlineSingle_Meths_pos m n:
+    WfBaseModule m ->
+    WfBaseModule (BaseMod (getRegisters m) (getRules m) (inlineSingle_Meths_pos (getMethods m) n)).
+  Proof.
+    intros.
+    assert (WfMod m) as P1;[constructor; auto|apply _WfMod_getFlat in P1].
+    unfold getFlat in P1; simpl in *.
+    specialize (TraceInclusion_inlineSingle_pos_Meths P1 n) as TMP; dest.
+    inversion H0; auto.
+  Qed.
+
+  Definition inlineSingle_Meths_pos_BaseModuleWf (m : BaseModuleWf) n :=
+    Build_BaseModuleWf (WfBaseMod_inlineSingle_Meths_pos n (wfBaseModule m)).
+
+  Theorem TraceInclusion_inlineSingle_pos_Meths_Wf (m : BaseModuleWf) n :
+    TraceInclusion m (inlineSingle_Meths_pos_BaseModuleWf m n).
+  Proof.
+    specialize (_TraceInclusion_flatten_r m) as P1.
+    specialize (wfMod (flattened_ModWf m)) as P2.
+    simpl in *; unfold flatten, getFlat in *; simpl in *.
+    specialize (TraceInclusion_inlineSingle_pos_Meths P2 n) as TMP; dest.
+    eauto using TraceInclusion_trans.
+  Qed.
+
   Theorem TraceInclusion_inlineAll_pos_Meths regs rules meths:
     (WfMod (Base (BaseMod regs rules meths))) ->
     (WfMod (Base (BaseMod regs rules (inlineAll_Meths meths)))) /\
@@ -3233,6 +3564,30 @@ Section inline_all_all.
     eapply TraceInclusion_trans; eauto.
   Qed.
 
+  Lemma WfBaseMod_inlineAll_Meths m :
+    WfBaseModule m ->
+    WfBaseModule (BaseMod (getRegisters m) (getRules m) (inlineAll_Meths (getMethods m))).
+  Proof.
+    intros.
+    assert (WfMod m) as P1;[constructor; auto|apply _WfMod_getFlat in P1].
+    unfold getFlat in P1; simpl in *.
+    specialize (TraceInclusion_inlineAll_pos_Meths P1) as TMP; dest.
+    inversion H0; auto.
+  Qed.
+
+  Definition inlineAll_Meths_BaseModuleWf (m : BaseModuleWf) :=
+    Build_BaseModuleWf (WfBaseMod_inlineAll_Meths (wfBaseModule m)).
+
+  Theorem TraceInclusion_inlineAll_pos_Meths_Wf (m : BaseModuleWf) :
+    TraceInclusion m (inlineAll_Meths_BaseModuleWf m).
+  Proof.
+    specialize (_TraceInclusion_flatten_r m) as P1.
+    specialize (wfMod (flattened_ModWf m)) as P2.
+    simpl in *; unfold flatten, getFlat in *; simpl in *.
+    specialize (TraceInclusion_inlineAll_pos_Meths P2) as TMP; dest.
+    eauto using TraceInclusion_trans.
+  Qed.
+  
   Theorem TraceInclusion_inlineAll_pos regs rules meths:
     (WfMod (Base (BaseMod regs rules meths))) ->
     (WfMod (Base (inlineAll_All regs rules meths))) /\
@@ -3244,6 +3599,30 @@ Section inline_all_all.
     pose proof (TraceInclusion_inlineAll_pos_Rules WfH2) as [WfH3 P3].
     split; auto.
     eapply TraceInclusion_trans; eauto.
+  Qed.
+
+  Lemma WfBaseMod_inlineAll_All m :
+    WfBaseModule m ->
+    WfBaseModule (inlineAll_All (getRegisters m) (getRules m) (getMethods m)).
+  Proof.
+    intros.
+    assert (WfMod m) as P1;[constructor; auto|apply _WfMod_getFlat in P1].
+    unfold getFlat in P1; simpl in *.
+    specialize (TraceInclusion_inlineAll_pos P1) as TMP; dest.
+    inversion H0; auto.
+  Qed.
+
+  Definition inlineAll_All_BaseModuleWf (m : BaseModuleWf) :=
+    Build_BaseModuleWf (WfBaseMod_inlineAll_All (wfBaseModule m)).
+
+  Theorem TraceInclusion_inlineAll_pos_Wf (m : BaseModuleWf) :
+    TraceInclusion m (inlineAll_All_BaseModuleWf m).
+  Proof.
+    specialize (_TraceInclusion_flatten_r m) as P1.
+    specialize (wfMod (flattened_ModWf m)) as P2.
+    simpl in *; unfold flatten, getFlat in *; simpl in *.
+    specialize (TraceInclusion_inlineAll_pos P2) as TMP; dest.
+    eauto using TraceInclusion_trans.
   Qed.
 End inline_all_all.
 
@@ -4967,6 +5346,14 @@ Proof.
     apply PPlusStrongTraceInclusion_inlining_Rules_l; auto.
 Qed.
 
+Theorem TraceInclusion_inlining_Rules_Wf_l {f} {m : BaseModuleWf} rn
+        (inMeths: In f (getMethods m)):
+  TraceInclusion (inlineSingle_Rule_BaseModuleWf rn inMeths) m.
+Proof.
+  simpl; apply TraceInclusion_inlining_Rules_l; eauto.
+  constructor; apply wfBaseModule.
+Qed.
+
 Lemma inlineSingle_Meth_in_list_body fb f gn l:
   (fst f) <> gn->
   In (gn, fb) (inlineSingle_Meth_in_list f gn l) ->
@@ -5461,6 +5848,14 @@ Proof.
     apply PPlusStrongTraceInclusion_inlining_Meths_l; auto.
 Qed.
 
+Theorem TraceInclusion_inlining_Meths_Wf_l {f} {m : BaseModuleWf} rn
+        (inMeths: In f (getMethods m)):
+  TraceInclusion (inlineSingle_Meth_BaseModuleWf rn inMeths) m.
+Proof.
+  simpl; apply TraceInclusion_inlining_Meths_l; eauto.
+  constructor; apply wfBaseModule.
+Qed.
+
 Theorem inline_meth_transform_l f regs rules meths:
   (WfMod (Base (BaseMod regs rules meths))) ->
   In f meths ->
@@ -5482,6 +5877,17 @@ Proof.
     apply TraceInclusion_refl.
 Qed.
 
+Theorem inline_meth_transform_Wf_l {f} {m : BaseModuleWf} i (inMeths : In f (getMethods m)):
+    TraceInclusion (inline_nth_Meth_BaseModuleWf i inMeths) m.
+Proof.
+  intros; simpl.
+  specialize (_TraceInclusion_flatten_l m) as P1.
+  specialize (wfMod (flattened_ModWf m)) as P2; simpl in *.
+  unfold flatten, getFlat in *; simpl in *.
+  specialize (inline_meth_transform_l f P2 inMeths i) as P3.
+  eauto using TraceInclusion_trans.
+Qed.
+
 Theorem inline_rule_transform_l f regs rules meths:
   (WfMod (Base (BaseMod regs rules meths))) ->
   In f meths ->
@@ -5501,6 +5907,17 @@ Proof.
   - apply Nat.nlt_ge in n.
     rewrite inlineSingle_transform_gt; auto.
     apply TraceInclusion_refl.
+Qed.
+
+Theorem inline_rule_transform_Wf_l {f} {m : BaseModuleWf} i (inMeths : In f (getMethods m)):
+    TraceInclusion (inline_nth_Rule_BaseModuleWf i inMeths) m.
+Proof.
+  intros; simpl.
+  specialize (_TraceInclusion_flatten_l m) as P1.
+  specialize (wfMod (flattened_ModWf m)) as P2; simpl in *.
+  unfold flatten, getFlat in *; simpl in *.
+  specialize (inline_rule_transform_l f P2 inMeths i) as P3.
+  eauto using TraceInclusion_trans.
 Qed.
 
 Section inlineSingle_nth_l.
@@ -5536,6 +5953,28 @@ Section inlineSingle_nth_l.
   Qed.
 End inlineSingle_nth_l.
 
+Theorem inline_meth_fold_right_Wf_l {f} {m : BaseModuleWf} xs (inMeth : In f (getMethods m)):
+  TraceInclusion (inline_all_Meth_BaseModuleWf xs inMeth) m.
+Proof.
+  specialize (_TraceInclusion_flatten_l m) as P1.
+  simpl in *; unfold flatten, getFlat in P1; simpl in *.
+  assert (WfMod m) as TMP;[constructor; apply wfBaseModule
+                          |specialize (_WfMod_getFlat TMP) as P2; clear TMP].
+  specialize (inline_meth_fold_right_l f P2 xs inMeth) as P3.
+  eauto using TraceInclusion_trans.
+Qed.
+
+Theorem inline_rule_fold_right_Wf_l {f} {m : BaseModuleWf} xs (inMeth : In f (getMethods m)):
+  TraceInclusion (inline_all_Rule_BaseModuleWf xs inMeth) m.
+Proof.
+  specialize (_TraceInclusion_flatten_l m) as P1.
+  simpl in *; unfold flatten, getFlat in P1; simpl in *.
+  assert (WfMod m) as TMP;[constructor; apply wfBaseModule
+                          |specialize (_WfMod_getFlat TMP) as P2; clear TMP].
+  specialize (inline_rule_fold_right_l f P2 xs inMeth) as P3.
+  eauto using TraceInclusion_trans.
+Qed.
+
 Theorem TraceInclusion_inline_BaseModule_rules_l regs rules meths f:
   (WfMod (Base (BaseMod regs rules meths))) ->
   In f meths ->
@@ -5547,6 +5986,18 @@ Proof.
   specialize (WfMod_inline_all_Rule _ (0 upto (length rules)) H0 H) as P2.
   repeat rewrite map_fold_right_eq in *.
   assumption.
+Qed.
+
+Theorem TraceInclusion_inline_BaseModule_rules_Wf_l {f} {m : BaseModuleWf}
+        (inMeth : In f (getMethods m)):
+  TraceInclusion (inline_BaseModule_rules_BaseModuleWf inMeth) m.
+Proof.
+  specialize (_TraceInclusion_flatten_l m) as P1.
+  simpl in *; unfold flatten, getFlat in P1; simpl in *.
+  assert (WfMod m) as TMP;[constructor; apply wfBaseModule
+                          |specialize (_WfMod_getFlat TMP) as P2; clear TMP].
+  specialize (TraceInclusion_inline_BaseModule_rules_l f P2 inMeth) as P3.
+  eauto using TraceInclusion_trans.
 Qed.
 
 Theorem TraceInclusion_inline_BaseModule_meths_l regs rules meths f:
@@ -5561,6 +6012,18 @@ Proof.
   assumption.
 Qed.
 
+Theorem TraceInclusion_inline_BaseModule_meths_Wf_l {f} {m : BaseModuleWf}
+        (inMeth : In f (getMethods m)):
+  TraceInclusion (inline_BaseModule_meths_BaseModuleWf inMeth) m.
+Proof.
+  specialize (_TraceInclusion_flatten_l m) as P1.
+  simpl in *; unfold flatten, getFlat in P1; simpl in *.
+  assert (WfMod m) as TMP;[constructor; apply wfBaseModule
+                          |specialize (_WfMod_getFlat TMP) as P2; clear TMP].
+  specialize (TraceInclusion_inline_BaseModule_meths_l f P2 inMeth) as P3.
+  eauto using TraceInclusion_trans.
+Qed.
+
 Theorem TraceInclusion_inline_BaseModule_all_l regs rules meths f:
   (WfMod (Base (BaseMod regs rules meths))) ->
   In f meths ->
@@ -5573,6 +6036,17 @@ Proof.
   specialize (TraceInclusion_inline_BaseModule_meths_l f P2 H0) as P3.
   repeat rewrite map_fold_right_eq in *.
   apply (TraceInclusion_trans P3 P1).
+Qed.
+
+Theorem TraceInclusion_inline_BaseModule_all_Wf_l {f} {m : BaseModuleWf}
+        (inMeth : In f (getMethods m)):
+  TraceInclusion (inlineSingle_BaseModuleWf inMeth) m.
+Proof.
+  specialize (_TraceInclusion_flatten_l m) as P1.
+  specialize (wfMod (flattened_ModWf m)) as P2.
+  simpl in *; unfold flatten, getFlat in *; simpl in *.
+  specialize (TraceInclusion_inline_BaseModule_all_l P2 inMeth) as P3.
+  eauto using TraceInclusion_trans.
 Qed.
 
 Section inline_all_all_l.
@@ -5594,6 +6068,16 @@ Section inline_all_all_l.
       eapply nth_error_In; eauto.
   Qed.
 
+  Theorem TraceInclusion_inlineSingle_pos_Rules_Wf_l (m : BaseModuleWf) n :
+    TraceInclusion (inlineSingle_Rules_pos_BaseModuleWf m n) m.
+  Proof.
+    specialize (_TraceInclusion_flatten_l m) as P1.
+    specialize (wfMod (flattened_ModWf m)) as P2.
+    simpl in *; unfold flatten, getFlat in *; simpl in *.
+    specialize (TraceInclusion_inlineSingle_pos_Rules_l P2 n) as TMP; dest.
+    eauto using TraceInclusion_trans.
+  Qed.
+  
   Theorem TraceInclusion_inlineAll_pos_Rules_l regs rules meths:
     (WfMod (Base (BaseMod regs rules meths))) ->
     (WfMod (Base (BaseMod regs (inlineAll_Rules meths rules) meths))) /\
@@ -5608,6 +6092,16 @@ Section inline_all_all_l.
     destruct n; simpl in *; auto.
     split; auto.
     eapply TraceInclusion_trans; eauto.
+  Qed.
+  
+  Theorem TraceInclusion_inlineAll_pos_Rules_Wf_l (m : BaseModuleWf) :
+    TraceInclusion (inlineAll_Rules_BaseModuleWf m) m.
+  Proof.
+    specialize (_TraceInclusion_flatten_l m) as P1.
+    specialize (wfMod (flattened_ModWf m)) as P2.
+    simpl in *; unfold flatten, getFlat in *; simpl in *.
+    specialize (TraceInclusion_inlineAll_pos_Rules_l P2) as TMP; dest.
+    eauto using TraceInclusion_trans.
   Qed.
   
   Theorem TraceInclusion_inlineSingle_pos_Meths_l regs rules meths:
@@ -5627,7 +6121,17 @@ Section inline_all_all_l.
     - apply TraceInclusion_inline_BaseModule_meths_l; auto.
       eapply nth_error_In; eauto.
   Qed.
-
+  
+  Theorem TraceInclusion_inlineSingle_pos_Meths_Wf_l (m : BaseModuleWf) n :
+    TraceInclusion (inlineSingle_Meths_pos_BaseModuleWf m n) m.
+  Proof.
+    specialize (_TraceInclusion_flatten_l m) as P1.
+    specialize (wfMod (flattened_ModWf m)) as P2.
+    simpl in *; unfold flatten, getFlat in *; simpl in *.
+    specialize (TraceInclusion_inlineSingle_pos_Meths_l P2 n) as TMP; dest.
+    eauto using TraceInclusion_trans.
+  Qed.
+  
   Theorem TraceInclusion_inlineAll_pos_Meths_l regs rules meths:
     (WfMod (Base (BaseMod regs rules meths))) ->
     (WfMod (Base (BaseMod regs rules (inlineAll_Meths meths)))) /\
@@ -5643,7 +6147,17 @@ Section inline_all_all_l.
     split; auto.
     eapply TraceInclusion_trans; eauto.
   Qed.
-
+  
+  Theorem TraceInclusion_inlineAll_pos_Meths_Wf_l (m : BaseModuleWf) :
+    TraceInclusion (inlineAll_Meths_BaseModuleWf m) m.
+  Proof.
+    specialize (_TraceInclusion_flatten_l m) as P1.
+    specialize (wfMod (flattened_ModWf m)) as P2.
+    simpl in *; unfold flatten, getFlat in *; simpl in *.
+    specialize (TraceInclusion_inlineAll_pos_Meths_l P2) as TMP; dest.
+    eauto using TraceInclusion_trans.
+  Qed.
+  
   Theorem TraceInclusion_inlineAll_pos_l regs rules meths:
     (WfMod (Base (BaseMod regs rules meths))) ->
     (WfMod (Base (inlineAll_All regs rules meths))) /\
@@ -5655,6 +6169,16 @@ Section inline_all_all_l.
     pose proof (TraceInclusion_inlineAll_pos_Rules_l WfH2) as [WfH3 P3].
     split; auto.
     eapply TraceInclusion_trans; eauto.
+  Qed.
+
+  Theorem TraceInclusion_inlineAll_pos_Wf_l (m : BaseModuleWf) :
+    TraceInclusion (inlineAll_All_BaseModuleWf m) m.
+  Proof.
+    specialize (_TraceInclusion_flatten_l m) as P1.
+    specialize (wfMod (flattened_ModWf m)) as P2.
+    simpl in *; unfold flatten, getFlat in *; simpl in *.
+    specialize (TraceInclusion_inlineAll_pos_l P2) as TMP; dest.
+    eauto using TraceInclusion_trans.
   Qed.
 End inline_all_all_l.
 
